
\begin{problem}{5a.1}
Demonstrate that \[\left( \frac{f_{Q}}{\sigma_{Q}} \right)^{2} = \left( \frac{f_{B}}{\sigma_{B}} \right)^{2} + \mathrm{IR}^{2}\]
\end{problem}

\begin{proof}[Solution]
We start with the right-hand side and expand it using (5A.14).
\begin{align*}
\left( \frac{f_{B}}{\sigma_{B}} \right)^{2} + \mathrm{IR}^{2} &= \left( \frac{f_{B}}{\sigma_{B}} \right)^{2} + \left( \frac{f_{Q}}{\sigma_{Q}} \right)^{2} \left( \frac{\omega_{Q}}{\sigma_{Q}} \right)^{2}\\
&= \frac{f_{B}^{2}}{\sigma_{B}^{2}} + \frac{f_{Q}^{2}}{\sigma_{Q}^{2}}\frac{\sigma_{Q}^{2} - \beta_{Q}^{2}\sigma_{B}^{2}}{\sigma_{Q}^{2}}\\
&= \frac{f_{B}^{2}}{\sigma_{B}^{2}} + \frac{f_{Q}^{2}}{\sigma_{Q}^{2}} - \beta_{Q}^{2}\frac{f_{Q}^{2}\sigma_{B}^{2}}{\sigma_{Q}^{4}}\\
&= \frac{f_{B}^{2}}{\sigma_{B}^{2}} + \frac{f_{Q}^{2}}{\sigma_{Q}^{2}} - \frac{f_{B}^{2}\sigma_{Q}^{4}}{f_{Q}^{2}\sigma_{B}^{4}}\frac{f_{Q}^{2}\sigma_{B}^{2}}{\sigma_{Q}^{4}} &(2A.37)\\
&= \frac{f_{B}^{2}}{\sigma_{B}^{2}} + \frac{f_{Q}^{2}}{\sigma_{Q}^{2}} - \frac{f_{B}^{2}}{\sigma_{B}^{2}}\\
&= \frac{f_{Q}^{2}}{\sigma_{Q}^{2}}.
\end{align*}
\end{proof}


\begin{problem}{5a.2}
Demonstrate that \[\beta_{Q} = \frac{\beta_{C} \cdot f_{B}}{\beta_{C} \cdot f_{B} + \alpha_{C}}\] Note that $\beta_{C} = (\sigma_{C}/\sigma_{B})^{2}$. In the absence of benchmark timing, i.e., if $f_{B} = \mu_{B}$, the alpha of portfolio $C$ is the key to determining the beta of portfolio $Q$.
\end{problem}

\begin{proof}[Solution]
This follows straightforwardly from (2A.38):
\begin{align*}
\beta_{Q} &= \frac{\beta_{C} \cdot f_{B}}{f_{C}}\\
&= \frac{\beta_{C} \cdot f_{B}}{\beta_{C} \cdot f_{B} + \alpha_{C}}.
\end{align*}
\end{proof}