\begin{problem}{10.1a}
Using Eq.\ (10A.21), what is the variance of the combined forecast? What is its covariance with the return? Remember that the combined forecast is simply a linear combination of signals. We know the volatilities and correlations of all the signals, and we know the correlation of each signal with the return.

Verify Eq.\ (10A.23) for the IC of the combined forecast. Demonstrate that when $K = 2$, it reduces to Eq.\ (10.27) in the main text of the chapter. 
\end{problem}

\begin{proof}[Solution]
Eq.\ (10A.21) states that \[\phi = \omega \cdot \IC_{\g}^{T} \cdot \brho_{\g}^{-1} \cdot \z.\] Note that $\var{\z} = \brho_{\g}$ by Eq.\ (10A.18). Hence, the variance of the combined forecast is
\begin{align*}
\var{\phi} &= \omega^{2} \cdot \IC_{\g}^{T} \cdot \brho_{\g}^{-1} \cdot \var{\z} \cdot \brho_{\g}^{-1} \cdot \IC_{\g}\\
&= \omega^{2} \cdot \IC_{\g}^{T} \cdot \brho_{\g}^{-1} \cdot \brho_{\g} \cdot \brho_{\g}^{-1} \cdot \IC_{\g}\\
&= \omega^{2} \cdot \IC_{\g}^{T} \cdot \brho_{\g}^{-1} \cdot \IC_{\g}.
\end{align*}
The covariance of the combined forecast with the return is
\begin{align*}
\cov{\phi, r} &= \cov{\omega \cdot \IC_{\g}^{T} \cdot \brho_{\g}^{-1} \cdot \z, r}\\
&= \omega \cdot \IC_{\g}^{T} \cdot \brho_{\g}^{-1} \cdot \cov{\z, r}\\
&= \omega \cdot \IC_{\g}^{T} \cdot \brho_{\g}^{-1} \cdot \omega \cdot \IC_{\g}\\
&= \omega^{2} \cdot \IC_{\g}^{T} \cdot \brho_{\g}^{-1} \cdot \IC_{\g}.
\end{align*}
Therefore, the IC of the combined forecast is
\begin{align*}
\mathrm{IC}_{\phi} &= \frac{\cov{\phi, r}}{\omega \cdot \std{\phi}}\\
&= \frac{\omega^{2} \cdot \IC_{\g}^{T} \cdot \brho_{\g}^{-1} \cdot \IC_{\g}}{\omega \cdot \sqrt{\omega^{2} \cdot \IC_{\g}^{T} \cdot \brho_{\g}^{-1} \cdot \IC_{\g}}}\\
&= \frac{\IC_{\g}^{T} \cdot \brho_{\g}^{-1} \cdot \IC_{\g}}{\sqrt{\IC_{\g}^{T} \cdot \brho_{\g}^{-1} \cdot \IC_{\g}}}\\
&= \sqrt{\IC_{\g}^{T} \cdot \brho_{\g}^{-1} \cdot \IC_{\g}}.
\end{align*}
This verifies Eq.\ (10A.23). We now demonstrate that when $K = 2$, it reduces to Eq.\ (10.27) in the main text of the chapter. We let \[\g = \begin{bmatrix}
g \\
g'
\end{bmatrix},
\] and $\rho = \corr{g, g'}$. Recall from Eq.\ (10A.25) that \[
\brho_{\g}^{-1} = \frac{1}{1 - \rho^{2}}
\begin{bmatrix}
1 & -\rho \\
-\rho & 1
\end{bmatrix}.
\] This makes
\begin{align*}
\IC_{\g}^{T} \cdot \brho_{\g}^{-1} \cdot \IC_{\g} &= \frac{1}{1 - \rho^{2}}
\begin{bmatrix}
\mathrm{IC}_{g} & \mathrm{IC}_{g'}
\end{bmatrix}
\begin{bmatrix}
1 & -\rho \\
-\rho & 1
\end{bmatrix}
\begin{bmatrix}
\mathrm{IC}_{g}\\
\mathrm{IC}_{g'}
\end{bmatrix}
\\
&= \frac{1}{1 - \rho^{2}} (\mathrm{IC}_{g}(\mathrm{IC}_{g} - \rho\mathrm{IC}_{g'}) + \mathrm{IC}_{g'}(\mathrm{IC}_{g'} - \rho\mathrm{IC}_{g})) \\
&= \frac{\mathrm{IC}_{g}^{2} - 2 \rho \mathrm{IC}_{g}\mathrm{IC}_{g'} + \mathrm{IC}_{g'}^{2}}{1 - \rho^{2}}.
\end{align*}
Hence, Eq.\ (10A.23) reduces to Eq.\ (10.27) from the main text of the chapter:
\[\mathrm{IC}_{\phi} = \sqrt{\frac{\mathrm{IC}_{g}^{2} - 2 \rho \mathrm{IC}_{g}\mathrm{IC}_{g'} + \mathrm{IC}_{g'}^{2}}{1 - \rho^{2}}}.\]
\end{proof}

